client.v
@@ -1,0 +1,91 @@
+From iris.program_logic Require Export weakestpre.
+From iris.heap_lang Require Export lang.
+From iris.proofmode Require Import tactics.
+From iris.heap_lang Require Import proofmode notation.
+From iris.algebra Require Import gset gmap excl agree frac.
+From iris.heap_lang.lib Require Export lock.
+From iris.heap_lang.lib Require Import par.
+From iris.bi.lib Require Import fractional.
+Require Import clh_lock.
+
+
+Definition read  : expr :=
+    λ: "l" "k" ,
+    let: "p" := init_proc #() in
+    request "l" "p";;
+    let: "v" := !"k" in
+    grant "p";;
+    "v".
+
+
+Definition simple_client : expr :=
+    let: "r" := ref #42 in
+    let: "lock" := init_lock #()in
+    (read "lock" "r") ||| (read "lock" "r").
+
+
+Section proof.
+Local Set Default Proof Using All.
+ Context `{!heapG Σ, !lockedG Σ, !stateG Σ, !spawnG Σ} (N : namespace).
+
+
+
+Lemma read_spec l γ3 k:
+  {{{isLock N  l (k ↦ #42) γ3}}}
+    read #l #k
+  {{{ v, RET v;  ⌜v = #42⌝ }}}.
+Proof.
+  iIntros (ϕ) "#HLock Hcont".
+  wp_pures.
+  wp_bind (init_proc _)%E.
+  wp_apply (init_proc_spec N (k ↦ #42)%I γ3).
+  { done. }
+  iIntros (p) "HProc".
+  iDestruct "HProc" as ( γ1 γ2 γ1' γ2') "HProc".
+  wp_pures.
+  wp_apply (request_spec N l _ (k ↦ #42)%I γ1 γ2 γ3 γ1' γ2' with "[HProc]").
+  { iFrame "#".  iFrame. }
+  iIntros "HPost".
+  iDestruct "HPost" as (γ1'' γ2'') "[HProc [HL HR]]".
+  wp_pures.
+  wp_load.
+  wp_pures.
+  wp_apply( grant_spec N _ (k ↦ #42)%I γ1 γ2 γ3 γ1'' γ2'' with "[-Hcont]").
+  {iFrame. }
+  iIntros "HProc".
+  wp_pures.
+  iApply "Hcont".
+  eauto.
+Qed.
+
+
+Lemma simple_spec :
+  {{{True}}}simple_client {{{p, RET p; ⌜p=(#42, #42)%V ⌝}}}.
+Proof.
+      iIntros (ϕ) "_ Hcont".
+      rewrite /simple_client.
+      wp_alloc r as "H".
+      wp_let.
+      wp_bind (init_lock _ )%E.
+      wp_apply (init_lock_spec N (r ↦ #42)%I with "[-Hcont]").
+      eauto with iFrame.
+      iIntros (l) "HLock".
+      iDestruct "HLock" as (γ3) "#HLock".
+      wp_pures.
+      iApply (wp_par (λ v , ⌜v=#42⌝)%I (λ v , ⌜v=#42⌝)%I).
+      - iApply (read_spec).
+        {iFrame "#". }
+        iNext.
+        iIntros (v) "H".
+        iFrame.
+      - iApply (read_spec).
+        {iFrame "#". }
+        iNext.
+        iIntros (v) "H".
+        iFrame.
+      - iIntros (v1 v2) "[-> ->]".
+        iNext.
+        iApply "Hcont".
+        eauto.
+Qed.
+
